Keeping only the two-index variant of RST

examples/lowstar_resources/Swap.fst
@@ -29,24 +29,40 @@ open LowStar.RST.Pointer
 
 let swap (#a:Type) (ptr1 ptr2:B.pointer a)
   : RST unit (ptr_resource ptr1 <*> ptr_resource ptr2)
+             (fun _ -> ptr_resource ptr1 <*> ptr_resource ptr2)
              (fun _ -> True)
              (fun h0 x h1 -> 
                 sel (ptr_view ptr1) h0 == sel (ptr_view ptr2) h1 /\
-                sel (ptr_view ptr2) h0 == sel (ptr_view ptr1) h1) =
-  let x = frame (star_includes_left (ptr_resource ptr2)) (ptr_read ptr1) in 
-  let y = frame (star_includes_right (ptr_resource ptr1)) (ptr_read ptr2) in 
-  frame (star_includes_left (ptr_resource ptr2)) (ptr_write ptr1 y);
-  frame (star_includes_right (ptr_resource ptr1)) (ptr_write ptr2 x)
+                sel (ptr_view ptr2) h0 == sel (ptr_view ptr1) h1) = 
+  let x = rst_frame #(ptr_resource ptr1 <*> ptr_resource ptr2) #_ #_
+                    #(fun _ -> ptr_resource ptr1 <*> ptr_resource ptr2)
+                    (ptr_resource ptr2) 
+                    (fun _ -> ptr_read ptr1) in 
+  let y = rst_frame #(ptr_resource ptr1 <*> ptr_resource ptr2) #_ #_
+                    #(fun _ -> ptr_resource ptr1 <*> ptr_resource ptr2)
+                    (ptr_resource ptr1) 
+                    (fun _ -> ptr_read ptr2) in 
+  rst_frame #(ptr_resource ptr1 <*> ptr_resource ptr2) #_ #_
+            #(fun _ -> ptr_resource ptr1 <*> ptr_resource ptr2)
+            (ptr_resource ptr2) 
+            (fun _ -> ptr_write ptr1 y);
+  rst_frame #(ptr_resource ptr1 <*> ptr_resource ptr2) #_ #_
+            #(fun _ -> ptr_resource ptr1 <*> ptr_resource ptr2)
+            (ptr_resource ptr1) 
+            (fun _ -> ptr_write ptr2 x)
+
+(* Doing a large even number of swaps *)
 
 val n_swap (#a:Type) (ptr1 ptr2:B.pointer a)
   : RST unit (ptr_resource ptr1 <*> ptr_resource ptr2)
+             (fun _ -> ptr_resource ptr1 <*> ptr_resource ptr2)
              (fun _ -> True)
              (fun h0 x h1 -> 
                 sel (ptr_view ptr1) h0 == sel (ptr_view ptr1) h1 /\
                 sel (ptr_view ptr2) h0 == sel (ptr_view ptr2) h1) 
 
 #reset-options "--max_fuel 0 --max_ifuel 0 --using_facts_from '* -LowStar.Monotonic -FStar.Monotonic.HyperHeap -FStar.Monotonic.HyperStack -FStar.Reflection -FStar.Tactics -FStar.ModifiesGen -FStar.HyperStack -FStar.Monotonic.Heap -LowStar.Buffer -FStar.Calc -LowStar.RST.reveal_star_inv' --z3cliopt smt.qi.eager_threshold=100"
-let n_swap' #a ptr1 ptr2 =
+let n_swap #a ptr1 ptr2 =
                              
   swap ptr1 ptr2; swap ptr1 ptr2; swap ptr1 ptr2; swap ptr1 ptr2;  
   swap ptr1 ptr2; swap ptr1 ptr2; swap ptr1 ptr2; swap ptr1 ptr2;
@@ -78,3 +94,43 @@ let n_swap' #a ptr1 ptr2 =
   swap ptr1 ptr2; swap ptr1 ptr2; swap ptr1 ptr2; swap ptr1 ptr2;
   swap ptr1 ptr2; swap ptr1 ptr2; swap ptr1 ptr2; swap ptr1 ptr2   // 100
 #reset-options
+
+(* Allocating two pointers, swapping them, and freeing the memory *)
+
+let alloc_swap_free (#a:Type) (x:a) (y:a)
+  : RST (a & a) (empty_resource)
+                (fun _ -> empty_resource)
+                (fun _ -> True)
+                (fun _ (x',y') _ -> x' == y /\ y' == x) = 
+  reveal_star ();
+  // allocating two pointers
+  let ptr1 = rst_frame 
+               #empty_resource #_ #_ #(fun ptr1 -> ptr_resource ptr1)
+               empty_resource 
+               (fun _ -> ptr_alloc x) in
+  let ptr2 = rst_frame 
+               #(ptr_resource ptr1) #_ #_ #(fun ptr2 -> ptr_resource ptr1 <*> ptr_resource ptr2)
+               (ptr_resource ptr1) 
+               (fun _ -> ptr_alloc y) in
+  // running the swap function
+  swap ptr1 ptr2;
+  // reading the values of the pointers after swapping them
+  let x' = rst_frame #(ptr_resource ptr1 <*> ptr_resource ptr2) #_ #_
+                     #(fun _ -> ptr_resource ptr1 <*> ptr_resource ptr2)
+                     (ptr_resource ptr2) 
+                     (fun _ -> ptr_read ptr1) in 
+  let y' = rst_frame #(ptr_resource ptr1 <*> ptr_resource ptr2) #_ #_
+                     #(fun _ -> ptr_resource ptr1 <*> ptr_resource ptr2)
+                     (ptr_resource ptr1) 
+                     (fun _ -> ptr_read ptr2) in 
+  // freeing the memory
+  rst_frame #(ptr_resource ptr1 <*> ptr_resource ptr2) #_ #_ 
+            #(fun _ -> ptr_resource ptr1)
+            (ptr_resource ptr1) 
+            (fun _ -> ptr_free ptr2);
+  rst_frame #(ptr_resource ptr1) #_ #_ 
+            #(fun _ -> empty_resource)
+            (empty_resource) 
+            (fun _ -> ptr_free ptr1);
+  // returning the swapped values of pointers
+  (x',y')
